generalize from list bool to arbitrary destination type

BasicSerializers.v
@@ -1,84 +1,28 @@
-Require Import List ZArith.
-Import ListNotations.
+Require Import ZArith.
 
 From StructTact Require Import StructTactics Fin.
 Require Fin Ascii.
 
-Require Import Cheerios.Core.
-Require Import Cheerios.Tactics.
-Require Import Cheerios.DeserializerMonad.
+From Cheerios Require Import Monoid Core Tactics DeserializerMonad.
 Import DeserializerNotations.
 
-Definition bool_serialize (b : bool) : list bool := [b].
-
-Definition bool_deserialize : deserializer bool :=
-  l <- get ;;
-  match l with
-  | [] => fail
-  | b :: l' => put l' ;; ret b
-  end.
-
-Lemma bool_serialize_deserialize_id :
-  serialize_deserialize_id_spec bool_serialize bool_deserialize.
-Proof.
-  destruct a; auto.
-Qed.
-
-Instance bool_Serializer : Serializer bool :=
-  {| serialize := bool_serialize;
-     deserialize := bool_deserialize;
-     serialize_deserialize_id := bool_serialize_deserialize_id
-  |}.
-
-
-(* This is about 2x less space-efficient than necessary, since it outputs two
-   bits for every "bit" in the input, but it's very easy to verify. *)
-Fixpoint positive_serialize (p : positive) : list bool :=
-  match p with
-  | xI p' => serialize true ++ serialize true ++ positive_serialize p'
-  | xO p' => serialize true ++ serialize false ++ positive_serialize p'
-  | xH => serialize false
-  end.
-
-(* This has to be implemented directly on the implementation of Deserializer.t
-   because it performs recursion on the underlying list of bits. *)
-Fixpoint positive_deserialize (l : list bool) : option (positive * list bool) :=
-  match l with
-  | [] => None
-  | continue :: l' =>
-    if continue
-    then match l' with
-         | [] => None
-         | bit :: l' => match positive_deserialize l' with None => None
-                       | Some (p, l') => Some ((if bit then xI else xO) p, l')
-                       end
-         end
-    else Some (xH, l')
-  end.
-
-Lemma positive_serialize_deserialize_id :
-  forall p bin, positive_deserialize (positive_serialize p ++ bin) = Some (p, bin).
-Proof.
-  induction p; simpl; intros; auto; rewrite IHp; auto.
-Qed.
-
-Instance positive_Serializer : Serializer positive :=
-  {| serialize := positive_serialize;
-     deserialize := positive_deserialize;
-     serialize_deserialize_id := positive_serialize_deserialize_id
-  |}.
+Section bin.
+  Variable bin : Type.
+  Context {mbin : Monoid bin}.
+  Context {sbool : Serializer bin bool}.
+  Context {spos : Serializer bin positive}.
 
 (* This is the first example of a "typical" serializer: it combines more
    primitive serializers (in this case, just for bool and positive) together in
    order to serialize a Z. *)
-Definition Z_serialize (z : Z) : list bool :=
+Definition Z_serialize (z : Z) : bin :=
   match z with
   | Z0 => serialize false
-  | Zpos p => serialize true ++ serialize true ++ serialize p
-  | Zneg p => serialize true ++ serialize false ++ serialize p
+  | Zpos p => serialize true +++ serialize true +++ serialize p
+  | Zneg p => serialize true +++ serialize false +++ serialize p
   end.
 
-Definition Z_deserialize : deserializer Z :=
+Definition Z_deserialize : deserializer bin Z :=
   tag <- deserialize ;;
   match tag with
   | true => sign <- deserialize ;;
@@ -88,28 +32,28 @@ Definition Z_deserialize : deserializer Z :=
 
 (* This proof is typical for serializing an algebraic datatype. Unfold the
    serializer and deserializer, then do a case analysis and call
-   serialize_deserialize_id_crush. *)
+   cheerios_crush. *)
 Lemma Z_serialize_deserialize_id :
   serialize_deserialize_id_spec Z_serialize Z_deserialize.
 Proof.
   unfold Z_serialize, Z_deserialize.
-  destruct a; serialize_deserialize_id_crush.
+  destruct a; cheerios_crush.
 Qed.
 
-Instance Z_Serializer : Serializer Z :=
+Global Instance Z_Serializer : Serializer bin Z :=
   {| serialize := Z_serialize;
      deserialize := Z_deserialize;
      serialize_deserialize_id := Z_serialize_deserialize_id
   |}.
 
 
-Definition N_serialize (n : N) : list bool :=
+Definition N_serialize (n : N) : bin :=
   match n with
   | N0 => serialize false
-  | Npos p => serialize true ++ serialize p
+  | Npos p => serialize true +++ serialize p
   end.
 
-Definition N_deserialize : deserializer N :=
+Definition N_deserialize : deserializer bin N :=
   tag <- deserialize ;;
   match tag with
   | false => ret N0
@@ -120,10 +64,10 @@ Lemma N_serialize_deserialize_id :
   serialize_deserialize_id_spec N_serialize N_deserialize.
 Proof.
   unfold N_serialize, N_deserialize.
-  destruct a; serialize_deserialize_id_crush.
+  destruct a; cheerios_crush.
 Qed.
 
-Instance N_Serializer : Serializer N :=
+Global Instance N_Serializer : Serializer bin N :=
   {| serialize := N_serialize;
      deserialize := N_deserialize;
      serialize_deserialize_id := N_serialize_deserialize_id
@@ -132,23 +76,23 @@ Instance N_Serializer : Serializer N :=
 
 (* The other main way to define a serializer is to use an isomorphism to another
    type that is already serializable. *)
-Definition nat_serialize (n : nat) : list bool := serialize (N.of_nat n).
+Definition nat_serialize (n : nat) : bin := serialize (N.of_nat n).
 
-Definition nat_deserialize : deserializer nat := N.to_nat <$> deserialize.
+Definition nat_deserialize : deserializer bin nat := N.to_nat <$> deserialize.
 
 (* This proof is typical for serializers defined by converting to and from a
    type that is already serializable. Unfold the serializer and deserializer,
-   call serialize_deserialize_id_crush, and then use the proof that the
+   call cheerios_crush, and then use the proof that the
    conversion functions are inverses. *)
 Lemma nat_serialize_deserialize_id :
   serialize_deserialize_id_spec nat_serialize nat_deserialize.
 Proof.
   unfold nat_serialize, nat_deserialize.
-  serialize_deserialize_id_crush.
+  cheerios_crush.
   now rewrite Nnat.Nat2N.id.
 Qed.
 
-Instance nat_Serializer : Serializer nat :=
+Global Instance nat_Serializer : Serializer bin nat :=
   {| serialize := nat_serialize;
      deserialize := nat_deserialize;
      serialize_deserialize_id := nat_serialize_deserialize_id
@@ -156,10 +100,10 @@ Instance nat_Serializer : Serializer nat :=
 
 
 (* Serializer for the standard library's Fin.t based on converting to nat. *)
-Definition Fin_serialize {n} (x : Fin.t n) : list bool :=
+Definition Fin_serialize {n} (x : Fin.t n) : bin :=
   serialize (proj1_sig (Fin.to_nat x)).
 
-Definition Fin_deserialize {n} : deserializer (Fin.t n) :=
+Definition Fin_deserialize {n} : deserializer bin (Fin.t n) :=
   m <- deserialize ;;
     match Fin.of_nat m n with
     | inleft x => ret x
@@ -178,11 +122,11 @@ Qed.
 Lemma Fin_serialize_deserialize_id n : serialize_deserialize_id_spec Fin_serialize (@Fin_deserialize n).
 Proof.
   unfold Fin_serialize, Fin_deserialize.
-  serialize_deserialize_id_crush.
+  cheerios_crush.
   now rewrite Fin_of_nat_to_nat.
 Qed.
 
-Instance Fin_Serializer n : Serializer (Fin.t n) :=
+Global Instance Fin_Serializer n : Serializer bin (Fin.t n) :=
   {| serialize := Fin_serialize;
      deserialize := Fin_deserialize;
      serialize_deserialize_id := Fin_serialize_deserialize_id n
@@ -190,10 +134,10 @@ Instance Fin_Serializer n : Serializer (Fin.t n) :=
 
 
 (* Serializer for StructTact's fin based on converting to nat. *)
-Definition fin_serialize {n} (x : fin n) : list bool :=
+Definition fin_serialize {n} (x : fin n) : bin :=
   serialize (fin_to_nat x).
 
-Definition fin_deserialize {n} : deserializer (fin n) :=
+Definition fin_deserialize {n} : deserializer bin (fin n) :=
   m <- deserialize ;;
     match fin_of_nat m n with
     | inleft x => ret x
@@ -203,33 +147,34 @@ Definition fin_deserialize {n} : deserializer (fin n) :=
 Lemma fin_serialize_deserialize_id n : serialize_deserialize_id_spec fin_serialize (@fin_deserialize n).
 Proof.
   unfold fin_serialize, fin_deserialize.
-  serialize_deserialize_id_crush.
+  cheerios_crush.
   now rewrite fin_of_nat_fin_to_nat.
 Qed.
 
-Instance fin_Serializer n : Serializer (fin n) :=
+Global Instance fin_Serializer n : Serializer bin (fin n) :=
   {| serialize := fin_serialize;
      deserialize := fin_deserialize;
      serialize_deserialize_id := fin_serialize_deserialize_id n
   |}.
 
 
-Definition ascii_serialize (a : Ascii.ascii) : list bool :=
+Definition ascii_serialize (a : Ascii.ascii) : bin :=
   serialize (Ascii.nat_of_ascii a).
 
-Definition ascii_deserialize : deserializer Ascii.ascii :=
+Definition ascii_deserialize : deserializer bin Ascii.ascii :=
   Ascii.ascii_of_nat <$> deserialize.
 
 Lemma ascii_serialize_deserialize_id :
   serialize_deserialize_id_spec ascii_serialize ascii_deserialize.
 Proof.
   unfold ascii_deserialize, ascii_serialize.
-  serialize_deserialize_id_crush.
+  cheerios_crush.
   now rewrite Ascii.ascii_nat_embedding.
 Qed.
 
-Instance ascii_Serializer : Serializer Ascii.ascii :=
+Global Instance ascii_Serializer : Serializer bin Ascii.ascii :=
   {| serialize := ascii_serialize;
      deserialize := ascii_deserialize;
      serialize_deserialize_id := ascii_serialize_deserialize_id
   |}.
+End bin.
