Combinators.v
@@ -1,12 +1,9 @@
-Require Import List.
+Require Import List ZArith.
 Import ListNotations.
 Require Vector String.
 
-Require Import Cheerios.Core.
-Require Import Cheerios.BasicSerializers.
-Require Import Cheerios.DeserializerMonad.
+From Cheerios Require Import Monoid Core BasicSerializers DeserializerMonad Tactics StringUtils.
 Import DeserializerNotations.
-Require Import Cheerios.Tactics.
 
 (* These functions are either missing obvious implicits, or have
    implicit arguments that are not marked "maximally inserted", which
@@ -17,21 +14,29 @@ Arguments option_map {_ _} _ _.
 Arguments Vector.nil {_}.
 Arguments Vector.cons {_} _ {_} _.
 
+Section bin.
+
+Variable bin : Type.
+Context {mbin : Monoid bin}.
+
+Context {sbool : Serializer bin bool}.
+Context {spos : Serializer bin positive}.
+
 Section combinators.
 
   (* This section gives instances for various type constructors, including pairs
     and lists. *)
   Variables A B : Type.
-  Variable sA : Serializer A.
-  Variable sB : Serializer B.
+  Variable sA : Serializer bin A.
+  Variable sB : Serializer bin B.
 
-  Definition option_serialize (x : option A) : list bool :=
+  Definition option_serialize (x : option A) : bin :=
     match x with
-    | Some a => serialize true ++ serialize a
+    | Some a => serialize true +++ serialize a
     | None => serialize false
     end.
 
-  Definition option_deserialize : deserializer (option A) :=
+  Definition option_deserialize : deserializer bin (option A) :=
     b <- deserialize ;;
     match b with
     | true => Some <$> deserialize
@@ -42,42 +47,42 @@ Section combinators.
     serialize_deserialize_id_spec option_serialize option_deserialize.
   Proof.
     unfold option_serialize, option_deserialize.
-    destruct a; serialize_deserialize_id_crush.
+    destruct a; cheerios_crush.
   Qed.
 
-  Global Instance option_Serializer : Serializer (option A) :=
+  Global Instance option_Serializer : Serializer bin (option A) :=
     {| serialize := option_serialize;
         deserialize := option_deserialize;
         serialize_deserialize_id := option_serialize_deserialize_id
     |}.
 
-  Definition pair_serialize (x : A * B) : list bool :=
-    let (a, b) := x in serialize a ++ serialize b.
+  Definition pair_serialize (x : A * B) : bin :=
+    let (a, b) := x in serialize a +++ serialize b.
 
-  Definition pair_deserialize : deserializer (A * B) :=
+  Definition pair_deserialize : deserializer bin (A * B) :=
     liftD2 pair.
 
   Lemma pair_serialize_deserialize_id :
     serialize_deserialize_id_spec pair_serialize pair_deserialize.
   Proof.
     unfold pair_serialize, pair_deserialize.
-    destruct a; serialize_deserialize_id_crush.
+    destruct a; cheerios_crush.
   Qed.
 
-  Global Instance pair_Serializer : Serializer (A * B) :=
+  Global Instance pair_Serializer : Serializer bin (A * B) :=
     {| serialize := pair_serialize;
         deserialize := pair_deserialize;
         serialize_deserialize_id := pair_serialize_deserialize_id
     |}.
 
 
-  Definition sum_serialize (x : A + B) : list bool :=
+  Definition sum_serialize (x : A + B) : bin :=
     match x with
-    | inl a => serialize true ++ serialize a
-    | inr b => serialize false ++ serialize b
+    | inl a => serialize true +++ serialize a
+    | inr b => serialize false +++ serialize b
     end.
 
-  Definition sum_deserialize : deserializer (A + B) :=
+  Definition sum_deserialize : deserializer bin (A + B) :=
     b <- deserialize ;;
     match b with
     | true => inl <$> deserialize
@@ -88,38 +93,38 @@ Section combinators.
     serialize_deserialize_id_spec sum_serialize sum_deserialize.
   Proof.
     unfold sum_serialize, sum_deserialize.
-    destruct a; serialize_deserialize_id_crush.
+    destruct a; cheerios_crush.
   Qed.
 
-  Global Instance sum_Serializer : Serializer (A + B) :=
+  Global Instance sum_Serializer : Serializer bin (A + B) :=
     {| serialize := sum_serialize;
         deserialize := sum_deserialize;
         serialize_deserialize_id := sum_serialize_deserialize_id
     |}.
 
 
-  Fixpoint list_serialize_rec (l : list A) : list bool :=
+  Fixpoint list_serialize_rec (l : list A) : bin :=
     match l with
-    | [] => []
-    | a :: l' => serialize a ++ list_serialize_rec l'
+    | [] => mempty
+    | a :: l' => serialize a +++ list_serialize_rec l'
     end.
 
-  Definition list_serialize (l : list A) : list bool :=
-    serialize (length l) ++ list_serialize_rec l.
+  Definition list_serialize (l : list A) : bin :=
+    serialize (length l) +++ list_serialize_rec l.
 
-  Fixpoint list_deserialize_rec (n : nat) : deserializer (list A) :=
+  Fixpoint list_deserialize_rec (n : nat) : deserializer bin (list A) :=
     match n with
     | 0 => ret []
     | S n' => cons <$> deserialize <*> list_deserialize_rec n'
     end.
 
-  Definition list_deserialize : deserializer (list A) :=
+  Definition list_deserialize : deserializer bin (list A) :=
     deserialize >>= list_deserialize_rec.
 
   Lemma list_serialize_deserialize_id_rec :
-    forall l bin, list_deserialize_rec (length l) (list_serialize_rec l ++ bin) = Some (l, bin).
+    forall l bin, list_deserialize_rec (length l) (list_serialize_rec l +++ bin) = Some (l, bin).
   Proof.
-    induction l; simpl; serialize_deserialize_id_crush.
+    induction l; simpl; cheerios_crush.
     now rewrite IHl.
   Qed.
 
@@ -127,24 +132,24 @@ Section combinators.
     serialize_deserialize_id_spec list_serialize list_deserialize.
   Proof.
     unfold list_serialize, list_deserialize.
-    serialize_deserialize_id_crush.
+    cheerios_crush.
     apply list_serialize_deserialize_id_rec.
   Qed.
 
-  Global Instance list_Serializer : Serializer (list A) :=
+  Global Instance list_Serializer : Serializer bin (list A) :=
     {| serialize := list_serialize;
-        deserialize := list_deserialize;
-        serialize_deserialize_id := list_serialize_deserialize_id
+       deserialize := list_deserialize;
+       serialize_deserialize_id := list_serialize_deserialize_id
     |}.
 
-  Fixpoint vector_serialize {n} (v : Vector.t A n) : list bool :=
+  Fixpoint vector_serialize {n} (v : Vector.t A n) : bin :=
     match v with
-    | Vector.nil => []
-    | Vector.cons a v' => serialize a ++ vector_serialize v'
+    | Vector.nil => mempty
+    | Vector.cons a v' => serialize a +++ vector_serialize v'
     end.
 
-  Fixpoint vector_deserialize {n} : deserializer (Vector.t A n) :=
-    match n as n0 return deserializer (Vector.t A n0) with
+  Fixpoint vector_deserialize {n} : deserializer bin (Vector.t A n) :=
+    match n as n0 return deserializer bin (Vector.t A n0) with
     | 0 => ret Vector.nil
     | S n' => a <- deserialize ;; v <- vector_deserialize ;; ret (Vector.cons a v)
     end.
@@ -153,62 +158,45 @@ Section combinators.
     forall n, serialize_deserialize_id_spec vector_serialize (@vector_deserialize n).
   Proof.
     induction n; intros.
-    - destruct a using Vector.case0. auto.
+    - destruct a using Vector.case0. simpl. rewrite mappend_mempty_l. auto.
     - destruct a using Vector.caseS'.
       simpl.
-      serialize_deserialize_id_crush.
+      cheerios_crush.
       now rewrite IHn.
   Qed.
 
-  Global Instance vector_Serializer n : Serializer (Vector.t A n) :=
+  Global Instance vector_Serializer n : Serializer bin (Vector.t A n) :=
     {| serialize := vector_serialize;
         deserialize := vector_deserialize;
         serialize_deserialize_id := vector_serialize_deserialize_id n
     |}.
-
 End combinators.
+
+Context {sascii : Serializer bin Ascii.ascii}.
 
 
 (* This has to go here because it depends on having a serializer for
    lists available. *)
 
-Fixpoint string_to_list s :=
-  match s with
-  | String.EmptyString => nil
-  | String.String c s' => c :: (string_to_list s')
-  end.
-
-Fixpoint list_to_string l :=
-  match l with
-  | nil => String.EmptyString
-  | h::l' => String.String h (list_to_string l')
-  end.
-
-Lemma string_to_list_to_string :
-  forall s, list_to_string (string_to_list s) = s.
-Proof.
-  induction s; auto; simpl.
-  now rewrite IHs.
-Qed.
-
 Definition string_serialize (s : String.string) :=
   serialize (string_to_list s).
 
-Definition string_deserialize : deserializer String.string :=
+Definition string_deserialize : deserializer bin String.string :=
   list_to_string <$> deserialize.
 
 Lemma string_serialize_deserialize_id :
   serialize_deserialize_id_spec string_serialize string_deserialize.
 Proof.
   unfold string_deserialize, string_serialize.
-  serialize_deserialize_id_crush.
+  cheerios_crush.
   now rewrite string_to_list_to_string.
 Qed.
 
-Instance string_Serializer : Serializer String.string :=
+Global Instance string_Serializer : Serializer bin String.string :=
   {| serialize := string_serialize;
      deserialize := string_deserialize;
      serialize_deserialize_id := string_serialize_deserialize_id
   |}.
 
 
+End bin.
