Core.v
@@ -1,26 +1,30 @@
 Require Import List.
 Import ListNotations.
 
+Require Import Cheerios.Monoid.
+
+
 Notation serialize_deserialize_id_spec s d :=
-  (forall a (bin : list bool), d (s a ++ bin) = Some (a, bin)).
+  (forall a bin, d (s a +++ bin) = Some (a, bin)).
 
 (* This is the class of serializable types, which is the main entrypoint to
    Cheerios. Instances are required to show that `deserialize` can correctly
    recognize a piece of `serialize`d data at the prefix of an arbitrary
    bitstream. *)
-Class Serializer (A : Type) : Type :=
+Class Serializer (bin : Type) {mbin : Monoid bin} (A : Type) : Type :=
   {
-    serialize : A -> list bool;
-    deserialize : list bool -> option (A * list bool);
+    serialize : A -> bin;
+    deserialize : bin -> option (A * bin);
     serialize_deserialize_id : serialize_deserialize_id_spec serialize deserialize
   }.
 
 (* In particular, if there is nothing else in the bitsream, then deserialize and
    serialize are inverses. *)
 Lemma serialize_deserialize_id_nil :
-  forall A (sA : Serializer A) a, deserialize (serialize a) = Some (a, []).
+  forall bin (mbin : Monoid bin) A (sA : Serializer bin A) a,
+    deserialize (serialize a) = Some (a, mempty).
 Proof.
   intros.
-  pose proof serialize_deserialize_id a [].
-  now rewrite app_nil_r in *.
+  pose proof serialize_deserialize_id a mempty.
+  now rewrite @mappend_mempty_r in *.
 Qed.
