Morphism.v
@@ -1,8 +1,6 @@
-Require Import List.
+Require Import List ZArith.
 Import ListNotations.
-Require Import Cheerios.Core.
-Require Import Cheerios.Combinators.
-Require Import Cheerios.Tactics.
+From Cheerios Require Import Monoid Core Combinators Tactics.
 
 (* A morphism between two serializable types A and B is a map A -> B that
    describes what happens if you serialize an A and then deserialize it *as a B*.
@@ -10,51 +8,61 @@ Require Import Cheerios.Tactics.
    for A and B. *)
 
 Notation triangle_spec f :=
-  (forall a bin, deserialize (serialize a ++ bin) = Some (f a, bin)).
+  (forall a bin, deserialize (serialize a +++ bin) = Some (f a, bin)).
 
-Class SerializerMorphism {A B : Type} (sA : Serializer A) (sB : Serializer B) : Type :=
+Class SerializerMorphism {A B bin : Type} {mbin : Monoid bin}
+      (sA : Serializer bin A) (sB : Serializer bin B) : Type :=
 {
   morphism : A -> B;
   triangle : triangle_spec morphism
 }.
 
-Lemma triangle_nil {A B sA sB} {m : @SerializerMorphism A B sA sB}  :
-  forall a, deserialize (serialize a) = Some (morphism a, []).
+Lemma triangle_nil {A B bin : Type} {mbin : Monoid bin}
+      {sA : Serializer bin A}
+      {sB : Serializer bin B}
+      {m : @SerializerMorphism A B bin mbin sA sB} :
+  forall a : A, deserialize (serialize a) = Some (morphism a, mempty).
 Proof.
   intros.
-  pose proof triangle a [].
-  now rewrite app_nil_r in *.
+  pose proof triangle a mempty.
+  now rewrite @mappend_mempty_r in *.
 Qed.
 
-(* Like Candy Crush if the candy was triangular. *)
-Ltac triangle_crush :=
-intros;
-deserializer_unfold;
-repeat rewrite ?app_assoc_reverse, ?serialize_deserialize_id, ?triangle;
-auto.
 
 Section morphism_combinators.
+  Variable bin : Type.
+  Variable mbin : Monoid bin.
+
+  Context {sbool : Serializer bin bool}.
+  Context {spos : Serializer bin positive}.
 
   Variables A B : Type.
-  Variable sA : Serializer A.
-  Variable sB : Serializer B.
+  Variable sA : Serializer bin A.
+  Variable sB : Serializer bin B.
   Variable m : SerializerMorphism sA sB.
 
-  Lemma option_triangle : triangle_spec (option_map morphism).
+  (* Unfortunately, typeclass resolution is not smart enough to use a version of this
+     hint that is universally quantified over the morphism, so you have to put this line
+     in every section where you want to define a combinator. *)
+
+  Hint Rewrite (triangle(SerializerMorphism := m)) : cheerios.
+
+  Lemma option_triangle :
+    triangle_spec (option_map morphism).
   Proof.
     simpl.
     unfold option_deserialize, option_serialize.
-    destruct a; triangle_crush.
+    destruct a; cheerios_crush.
   Qed.
 
-  Global Instance option_Morphism : @SerializerMorphism (option A) (option B) _ _ :=
+  Global Instance option_Morphism : @SerializerMorphism (option A) (option B) _ _ _ _ :=
     {|  morphism := option_map morphism;
         triangle := option_triangle
     |}.
 
 
   Variables C : Type.
-  Variable sC : Serializer C.
+  Variable sC : Serializer bin C.
 
 
   Definition pair_l_map (f : A -> B) (x : A * C) : B * C :=
@@ -64,10 +72,10 @@ Section morphism_combinators.
   Proof.
     simpl.
     unfold pair_deserialize, pair_serialize.
-    destruct a; triangle_crush.
+    destruct a; cheerios_crush.
   Qed.
 
-  Global Instance pair_l_Morphism : @SerializerMorphism (A * C) (B * C) _ _ :=
+  Global Instance pair_l_Morphism : @SerializerMorphism (A * C) (B * C) _ _ _ _ :=
     {|  morphism := pair_l_map morphism;
         triangle := pair_l_triangle
     |}.
@@ -80,10 +88,10 @@ Section morphism_combinators.
   Proof.
     simpl.
     unfold pair_deserialize, pair_serialize.
-    destruct a; triangle_crush.
+    destruct a; cheerios_crush.
   Qed.
 
-  Global Instance pair_r_Morphism : @SerializerMorphism (C * A) (C * B) _ _ :=
+  Global Instance pair_r_Morphism : @SerializerMorphism (C * A) (C * B) _ _ _ _ :=
     {| morphism := pair_r_map morphism;
         triangle := pair_r_triangle
     |}.
@@ -99,10 +107,10 @@ Section morphism_combinators.
   Proof.
     simpl.
     unfold sum_serialize, sum_deserialize.
-    destruct a; triangle_crush.
+    destruct a; cheerios_crush.
   Qed.
 
-  Global Instance sum_l_Morphism : @SerializerMorphism (A + C) (B + C) _ _ :=
+  Global Instance sum_l_Morphism : @SerializerMorphism (A + C) (B + C) _ _ _ _ :=
     {| morphism := sum_l_map morphism;
         triangle := sum_l_triangle
     |}.
@@ -118,21 +126,21 @@ Section morphism_combinators.
   Proof.
     simpl.
     unfold sum_serialize, sum_deserialize.
-    destruct a; triangle_crush.
+    destruct a; cheerios_crush.
   Qed.
 
-  Global Instance sum_r_Morphism : @SerializerMorphism (C + A) (C + B) _ _ :=
+  Global Instance sum_r_Morphism : @SerializerMorphism (C + A) (C + B) _ _ _ _ :=
     {| morphism := sum_r_map morphism;
         triangle := sum_r_triangle
     |}.
 
 
   Lemma list_triangle_rec:
-    forall (a : list A) (bin : list bool),
-      list_deserialize_rec B sB (length a) (list_serialize_rec A sA a ++ bin) =
-      Some (List.map morphism a, bin).
+    forall (a : list A) (data : bin),
+      list_deserialize_rec _ B sB (length a) (list_serialize_rec bin A sA a +++ data) =
+      Some (List.map morphism a, data).
   Proof.
-    induction a; simpl; triangle_crush.
+    induction a; simpl; cheerios_crush.
     now rewrite IHa.
   Qed.
 
@@ -140,11 +148,11 @@ Section morphism_combinators.
   Proof.
     simpl.
     unfold list_deserialize, list_serialize.
-    serialize_deserialize_id_crush.
+    cheerios_crush.
     apply list_triangle_rec.
   Qed.
 
-  Global Instance list_morphism : @SerializerMorphism (list A) (list B) _ _ :=
+  Global Instance list_morphism : @SerializerMorphism (list A) (list B) _ _ _ _ :=
     {| morphism := List.map morphism;
         triangle := list_triangle
     |}.
@@ -152,11 +160,11 @@ Section morphism_combinators.
 
   Lemma vector_triangle : forall n, triangle_spec (@Vector.map A B morphism n).
   Proof.
-    induction a; simpl in *; triangle_crush.
+    induction a; simpl in *; cheerios_crush.
     now rewrite IHa.
   Qed.
 
-  Global Instance vector_morphism n : @SerializerMorphism (Vector.t A n) (Vector.t B n) _ _ :=
+  Global Instance vector_morphism n : @SerializerMorphism (Vector.t A n) (Vector.t B n) _ _ _ _ :=
     {| morphism := Vector.map morphism;
         triangle := vector_triangle n
     |}.
