Examples/MorphismExample.v
@@ -3,19 +3,18 @@ Import ListNotations.
 Require Import Vectors.Vector.
 Import VectorNotations.
 
-Require Import Cheerios.Cheerios.
-Require Import Cheerios.Morphism.
+From Cheerios Require Import Cheerios ListBoolSerializers Morphism.
 
 (* As a simple example, we can prove that a serialized pair of two As can be
   deserialized as a vector of As of length 2. *)
 Section silly_example.
   Variables A : Type.
-  Variable sA : Serializer A.
+  Variable sA : Serializer (list bool) A.
 
   Definition pair_to_vector (x : A * A) : Vector.t A 2 := [fst x; snd x].
 
   Lemma A_to_vector_triangle : triangle_spec pair_to_vector.
   Proof.
-    destruct a; simpl; triangle_crush.
+    destruct a; simpl; cheerios_crush.
   Qed.
 End silly_example.
