ListBoolSerializers.v
@@ -1,0 +1,82 @@
+Require Import List ZArith.
+Import ListNotations.
+
+From Cheerios Require Import Monoid Core Tactics DeserializerMonad.
+Import DeserializerNotations.
+
+Definition bool_serialize (b : bool) : list bool := [b].
+
+Definition bool_deserialize : deserializer (list bool) bool :=
+  l <- get ;;
+  match l with
+  | [] => fail
+  | b :: l' => put l' ;; ret b
+  end%list.
+
+Lemma bool_serialize_deserialize_id :
+  serialize_deserialize_id_spec bool_serialize bool_deserialize.
+Proof.
+  destruct a; auto.
+Qed.
+
+Instance bool_Serializer : Serializer (list bool) bool :=
+  {| serialize := bool_serialize;
+     deserialize := bool_deserialize;
+     serialize_deserialize_id := bool_serialize_deserialize_id
+  |}.
+
+
+(* This is about 2x less space-efficient than necessary, since it outputs two
+   bits for every "bit" in the input, but it's very easy to verify. *)
+Fixpoint positive_serialize (p : positive) : list bool :=
+  match p with
+  | xI p' => serialize true +++ serialize true +++ positive_serialize p'
+  | xO p' => serialize true +++ serialize false +++ positive_serialize p'
+  | xH => serialize false
+  end.
+
+(* This has to be implemented directly on the implementation of Deserializer.t
+   because it performs recursion on the underlying list of bits. *)
+Fixpoint positive_deserialize (l : list bool) : option (positive * list bool) :=
+  match l with
+  | [] => None
+  | continue :: l' =>
+    if continue
+    then match l' with
+         | [] => None
+         | bit :: l' => match positive_deserialize l' with None => None
+                       | Some (p, l') => Some ((if bit then xI else xO) p, l')
+                       end
+         end
+    else Some (xH, l')
+  end%list.
+
+Lemma positive_serialize_deserialize_id :
+  forall p bin, positive_deserialize (positive_serialize p +++ bin) = Some (p, bin).
+Proof.
+  simpl.
+  induction p; simpl; intros; auto; rewrite IHp; auto.
+Qed.
+
+Instance positive_Serializer : Serializer (list bool) positive :=
+  {| serialize := positive_serialize;
+     deserialize := positive_deserialize;
+     serialize_deserialize_id := positive_serialize_deserialize_id
+  |}.
+
+Lemma fold_list_mappend : forall A (xs ys : list A), xs ++ ys = xs +++ ys.
+Proof. auto. Qed.
+
+Lemma serialize_deserialize_id_list_bool :
+  forall A (sA : Serializer (list bool) A)
+    (a : A) (bin : list bool),
+    deserialize (serialize a ++ bin) = Some (a, bin).
+Proof.
+  intros.
+  now rewrite fold_list_mappend, serialize_deserialize_id.
+Qed.
+
+Hint Rewrite
+     fold_list_mappend
+     @serialize_deserialize_id_list_bool
+  : cheerios.
