Monoid.v
@@ -1,0 +1,21 @@
+Require Import List String.
+Import ListNotations.
+
+Class Monoid (A : Type) : Type :=
+  { mempty : A;
+    mappend : A -> A -> A;
+    mappend_mempty_l : forall a, mappend mempty a = a;
+    mappend_mempty_r : forall a, mappend a mempty = a;
+    mappend_assoc : forall a b c, mappend (mappend a b) c = mappend a (mappend b c)
+  }.
+
+Notation "a +++ b" := (@mappend _ _ a b) (right associativity, at level 60) : monoid_scope.
+Open Scope monoid_scope.
+
+Instance ListMonoid {A} : Monoid (list A) :=
+  {| mempty := [];
+     mappend := @app A;
+     mappend_mempty_l := fun a => eq_refl;
+     mappend_mempty_r := @app_nil_r A;
+     mappend_assoc := @app_ass A
+  |}.
