StringUtils.v
@@ -1,0 +1,20 @@
+Require Import List String.
+
+Fixpoint string_to_list s :=
+  match s with
+  | String.EmptyString => nil
+  | String.String c s' => c :: (string_to_list s')
+  end.
+
+Fixpoint list_to_string l :=
+  match l with
+  | nil => String.EmptyString
+  | h::l' => String.String h (list_to_string l')
+  end.
+
+Lemma string_to_list_to_string :
+  forall s, list_to_string (string_to_list s) = s.
+Proof.
+  induction s; auto; simpl.
+  now rewrite IHs.
+Qed.
