Tactics.v
@@ -1,7 +1,6 @@
 Require Import List.
 
-Require Import Cheerios.Core.
-Require Import Cheerios.DeserializerMonad.
+From Cheerios Require Import Monoid Core DeserializerMonad.
 
 Ltac deserializer_unfold :=
   unfold (* list in reverse order so that dependencies get unfolded *)
@@ -20,7 +19,16 @@ Ltac deserializer_unfold :=
     ret
   in *.
 
-Ltac serialize_deserialize_id_crush :=
+Hint Rewrite
+     @mappend_assoc
+     @mappend_mempty_l
+     @mappend_mempty_r
+     @serialize_deserialize_id
+     @serialize_deserialize_id_nil
+  : cheerios.
+
+
+Ltac cheerios_crush :=
   intros; deserializer_unfold;
-  repeat rewrite ?app_assoc_reverse, ?serialize_deserialize_id;
+  autorewrite with cheerios;
   auto.
